on progresse vers le niveau 4

ILLVarInt.v
@@ -66,7 +66,7 @@ Module N_OT <: OrderedType.
     apply EQ. apply nat_compare_eq; assumption.
     apply LT. apply nat_compare_Lt_lt; assumption.
     apply GT. apply nat_compare_Gt_gt; assumption.
-    Defined.
+  Defined.
 
   Hint Immediate eq_sym.
   Hint Resolve eq_refl eq_trans lt_not_eq lt_trans.
@@ -132,10 +132,786 @@ Module M.
               match e with
                 | context C [(add (p'⊸q') ?env'')]  => 
                   let e' := context C [ env'' ] in
-                     impl_l ({ p' }) (e')  (p') (q')
+                    impl_l ({ p' }) (e')  (p') (q')
               end
         end
     end.
+
+
+  Require Import Setoid.
+
+  Function appears (under_plus:bool) (v:nat) (f:formula) {struct f} : bool := 
+    match f with
+      | Proposition n => EqNat.beq_nat n v
+      | Otimes f1 f2  | And f1 f2 => 
+        orb (appears under_plus v f1) (appears under_plus v f2)
+      | Oplus f1 f2 | Implies f1 f2 => 
+        if under_plus 
+          then  orb (appears under_plus v f1) (appears under_plus v f2) 
+          else false
+      | Bang f => appears under_plus v f
+      | Zero => true
+      | _ => false
+    end.
+
+  Definition exists_in_env f gamma := 
+    fold _ (fun k acc => orb (f k) acc) gamma false.
+
+  Definition appears_in_env v := exists_in_env (appears true v).
+
+  Lemma iter_bool_proper : forall v, Morphisms.Proper
+    (ILLVarInt.MILL.eq ==> Logic.eq ==> Logic.eq ==> Logic.eq)
+    (iter bool
+      (λ (k0 : formula) (acc : bool), (appears true v k0 || acc)%bool)).
+  Proof.
+    intros v.
+    red.
+    red.
+    intros x y H.
+    apply eq_is_eq in H.
+    subst.
+    red.
+    intros x y0 H.
+    subst.
+    red.
+    intros;subst;reflexivity.
+  Qed.
+
+  Lemma iter_transpose_nkey : forall v,MapsPtes.transpose_neqkey Logic.eq
+    (iter bool
+      (λ (k : formula) (acc : bool), (appears true v k || acc)%bool)).
+  Proof.
+    red.
+    intros v k k' e e' a _.
+    revert k' e' a.
+    induction e as [ | e].
+
+    simpl.
+    intros k' e'.
+    induction e' as [ | e'].
+    simpl;intros.
+    case(appears true v k);case (appears true v k');simpl;reflexivity. 
+    intros a.  
+    simpl.
+    rewrite <- IHe'.
+    case(appears true v k);case (appears true v k');simpl;reflexivity. 
+    intros k' e' a.
+    simpl.  
+    rewrite (IHe k' e').
+    f_equal.
+    case(appears true v k);simpl.
+    2:reflexivity.
+    clear.
+    induction e' as [|e'].
+    simpl.
+    auto with *.
+    simpl.
+    case (appears true v k');simpl;auto.
+  Qed.
+
+  Lemma appears_in_env_morph : ∀ v Γ Γ', Γ == Γ' -> appears_in_env v Γ = appears_in_env v Γ'.
+  Proof.
+    intros v Γ Γ' H.
+    unfold appears_in_env, exists_in_env,fold.
+    revert Γ' H.
+    apply MapsPtes.fold_rec. 
+    Focus 1.
+    intros m H Γ' H0.
+    rewrite H0 in H.
+    rewrite MapsPtes.fold_Empty.
+    reflexivity.
+    auto.
+    assumption.
+    Unfocus.
+
+    Focus 1.
+    intros k e a m' m'' H H0 H1 H2 Γ' H3.
+    rewrite MapsPtes.fold_Add.
+    f_equal.
+    apply H2.
+    reflexivity.
+    auto.
+    apply iter_bool_proper.
+    apply iter_transpose_nkey.
+    assumption.
+    Focus 1. 
+    intro.
+    rewrite <- H3.
+    apply H1.
+    Unfocus.
+  Qed.
+
+  Add Morphism appears_in_env with signature (Logic.eq ==> eq ==> Logic.eq) as morph_appears_in_env.
+    exact appears_in_env_morph.
+  Qed.
+
+  Lemma appears_false_is_appears_true : forall n p, appears false n p = true -> appears true n p = true.
+  Proof.
+    intros n p.
+    functional induction (appears false n p);simpl.
+    tauto.
+    intros H.  
+    rewrite Bool.orb_true_iff in H;destruct H.
+    rewrite IHb0;auto.
+    rewrite IHb1;auto with *.
+    intros H.  
+    rewrite Bool.orb_true_iff in H;destruct H.
+    rewrite IHb0;auto.
+    rewrite IHb1;auto with *.
+    intros H.  
+    rewrite Bool.orb_true_iff in H;destruct H.
+    rewrite IHb0;auto.
+    rewrite IHb1;auto with *.
+    discriminate.
+    intros H.  
+    rewrite Bool.orb_true_iff in H;destruct H.
+    rewrite IHb0;auto.
+    rewrite IHb1;auto with *.
+    discriminate.
+    auto.
+    reflexivity.
+    discriminate.
+  Qed.
+
+  Lemma exists_in_env_in : forall f φ Γ, φ∈Γ -> f φ = true -> exists_in_env f Γ = true.
+  Proof.
+    intros f φ Γ H H0.
+    revert φ H0 H.
+    unfold exists_in_env.
+    apply fold_rec_weak.
+
+    intros m m' a H H0 φ H1 H2.
+    rewrite <- H in H2;eauto.
+
+    intros φ H0 H.  
+    unfold mem in H.
+    rewrite MapsPtes.F.empty_a in H;assumption.
+
+    intros k a m H φ H0 H1.
+    destruct (mem_destruct _ _ _ H1) as [H2|H2].
+    apply eq_is_eq in H2;subst.
+    rewrite H0;reflexivity.
+    rewrite H with (φ:=φ).
+    auto with *.
+    assumption.
+    assumption.
+  Qed.
+
+  Lemma in_exists_in_env : forall f Γ, exists_in_env f Γ = true -> exists φ,φ∈Γ/\ f φ = true.
+  Proof.
+    intros f Γ.
+    unfold exists_in_env.
+    apply fold_rec_weak.
+
+    intros m m' a H H0 H1.
+    destruct (H0 H1) as [φ H2].
+    rewrite H in H2.
+    exists φ;assumption.
+
+    discriminate.
+
+    intros k a m H H0.
+    rewrite Bool.orb_true_iff in H0.
+    destruct H0.
+    exists k;split;auto.
+    apply add_is_mem;apply FormulaOrdered.eq_refl.
+    destruct (H H0) as [φ [H1 H2]].
+    exists φ;split.
+    apply mem_add_comm;assumption.
+    assumption.
+  Qed.
+
+  Lemma not_exists_in_env_in : forall f Γ, exists_in_env f Γ = false -> forall φ, φ∈Γ -> f φ = false.
+  Proof.
+    intros f Γ.
+    unfold exists_in_env.
+    apply fold_rec_weak.
+
+    intros m m' a H H0 H1 φ H2.
+    rewrite <- H in H2;auto.
+
+    intros H φ H0.
+    unfold mem in H0;rewrite MapsPtes.F.empty_a in H0.
+    discriminate.
+
+    intros k a m H H0 φ H1.
+    rewrite Bool.orb_false_iff in H0;destruct H0.
+    destruct (mem_destruct _ _ _ H1).
+    apply eq_is_eq in H3;subst.
+    assumption.
+    auto.
+  Qed.
+
+  Lemma in_not_exists_in_env : forall f Γ, (forall φ, φ∈Γ -> f φ = false) -> exists_in_env f Γ = false.
+  Proof.
+    intros f Γ.
+    unfold exists_in_env.
+    apply fold_rec_weak.
+
+    intros m m' a H H0 H1.
+    apply H0. 
+    intros φ H2.
+    rewrite H in H2;auto.
+
+    reflexivity.
+
+    intros k a m H H0.
+    rewrite H.
+    replace (f k) with false.
+    reflexivity.
+    symmetry.
+    apply H0.
+    apply add_is_mem.
+    apply FormulaOrdered.eq_refl.
+    intros φ H1.
+    apply H0.
+    apply mem_add_comm;assumption.
+  Qed.
+
+
+
+
+  Lemma exists_in_env_add : forall f φ Γ, exists_in_env f (φ::Γ) = ((f φ)|| (exists_in_env f Γ))%bool.
+  Proof.
+    intros f φ Γ.
+    case_eq (exists_in_env f (φ::Γ));intros Heq.
+    destruct (in_exists_in_env _ _ Heq) as [ψ [H1 H2]].
+    destruct (mem_destruct _ _ _ H1).
+    apply eq_is_eq in H;subst.
+    rewrite H2;reflexivity.
+    rewrite (exists_in_env_in _ _ _ H H2). 
+    auto with *.
+    assert (Heq':=not_exists_in_env_in _ _ Heq).
+    rewrite  in_not_exists_in_env.
+    rewrite Heq'.
+    reflexivity.
+    apply add_is_mem;apply FormulaOrdered.eq_refl.
+    intros φ0 H.
+    apply Heq';apply mem_add_comm;assumption.
+  Qed.
+  
+  Lemma appears_in_env_in_appears : forall n φ Γ, φ∈Γ -> appears true n φ = true -> appears_in_env n Γ=true.
+  Proof.
+    intros n φ Γ.
+
+    unfold appears_in_env.
+    intros H H0.
+    apply exists_in_env_in with φ;assumption.
+  Qed.
+
+  Lemma appears_in_env_false_add : 
+    forall n (Γ:t) φ, appears_in_env n (φ::Γ)  = false -> 
+      appears_in_env n Γ = false /\ appears true n φ = false.
+  Proof.
+    intros n Γ.
+
+    induction Γ using multiset_ind.
+
+    intros φ H0.
+    rewrite <- H in H0.
+    assert (H':=IHΓ1 _ H0).
+    rewrite H in H';assumption.
+
+    intros φ H.
+    case_eq (appears true n φ);intros Heq1.
+    unfold appears_in_env,exists_in_env,fold,add in H.
+    rewrite MapsPtes.F.empty_o in H.
+    symmetry in H.
+    rewrite MapsPtes.fold_add in H.
+    simpl in H.
+    rewrite Heq1 in H;discriminate.
+    auto.
+    apply iter_proper.
+    clear;repeat red.
+    intros x y H x0 y0 H0.
+    repeat red in H0.
+    apply eq_is_eq in H;subst;reflexivity.
+    apply iter_transpose_nkey.
+    rewrite MapsPtes.F.empty_in_iff;tauto.
+    auto.
+
+    intros φ H.
+    assert (H':=  not_exists_in_env_in _ _ H).
+    rewrite H' by (apply add_is_mem;apply FormulaOrdered.eq_refl).
+    split;auto.
+    apply in_not_exists_in_env.
+    intros φ0 H0.
+    apply H'.
+    apply mem_add_comm;assumption.
+  Qed.
+
+  Lemma appears_false_remove : ∀ n (Γ:t) φ, appears_in_env n Γ = false -> 
+    appears_in_env n (Γ\φ) = false.
+  Proof.
+    intros v Γ φ.
+    induction Γ using multiset_ind.
+
+    rewrite H in IHΓ1;assumption.
+
+    rewrite remove_empty;tauto.
+    intros H.
+    destruct (appears_in_env_false_add _ _ _ H) as [H1 H2];clear H.
+    apply in_not_exists_in_env.
+    intros φ0 H.
+    case (FormulaOrdered.eq_dec x φ);intro Heq.
+    rewrite remove_same_add in H by (symmetry;assumption).
+    apply not_exists_in_env_in with (Γ:=Γ);assumption.
+    rewrite remove_diff_add in H by (intro abs;elim Heq;rewrite abs;reflexivity).
+    generalize (mem_destruct _ _ _ H);intros [H3|H3].
+    apply eq_is_eq in H3;subst; assumption.
+    assert (H':=IHΓ H1).
+    apply not_exists_in_env_in with (Γ:=Γ\φ); assumption.
+  Qed.
+
+  Lemma appears_false_union : 
+    ∀ n Δ Δ', appears_in_env n (Δ∪Δ') = false -> 
+    appears_in_env n (Δ) = false /\ 
+    appears_in_env n (Δ') = false.
+  Proof.
+    intros n Δ Δ' H.
+    split;apply in_not_exists_in_env;intros.
+    apply not_exists_in_env_in with (Γ:=Δ∪Δ');try assumption.
+    apply mem_union_l;assumption.
+    apply not_exists_in_env_in with (Γ:=Δ∪Δ');try assumption.
+    apply mem_union_r;assumption.
+  Qed.
+
+  Lemma var_in_env : ∀ Γ φ n, (appears false n φ) = true -> appears_in_env n Γ = false -> Γ⊢φ -> False.
+  Proof.
+    intros Γ φ n H H0 H1.
+    revert H H0.
+
+    induction H1;intros  Heq1 Heq2;simpl in *;try discriminate.
+
+    Focus 1.
+    rewrite H in Heq2.
+    unfold appears_in_env,exists_in_env,fold,Maps'.fold in Heq2. simpl in Heq2.
+    apply appears_false_is_appears_true in Heq1.
+    rewrite Heq1 in Heq2.
+    discriminate Heq2.
+
+    Focus 1.
+    apply IHILL_proof2.
+    assumption.
+    assert (Heq2' := Heq2).
+    apply (appears_false_remove _ _ (p⊸q)) in Heq2.
+    rewrite H0 in Heq2.
+    apply appears_false_union in Heq2.
+    destruct Heq2.
+    apply in_not_exists_in_env.
+    intros φ H3.
+    destruct (mem_destruct _ _ _ H3) as [H4|H4].
+    apply eq_is_eq in H4;subst.
+    assert (appears true n (p⊸q) = false).
+    apply not_exists_in_env_in with (Γ:=Γ); assumption.
+    simpl in H4.
+    rewrite Bool.orb_false_iff in H4;intuition.
+    apply not_exists_in_env_in with (Γ:=Δ'); assumption.
+
+    Focus.
+    rewrite H in Heq2.
+    apply appears_false_union in Heq2;destruct Heq2.
+    rewrite Bool.orb_true_iff in Heq1;destruct Heq1.
+    apply IHILL_proof1;assumption.
+    apply IHILL_proof2;assumption.
+
+    Focus.
+    apply IHILL_proof.
+    assumption.
+    assert (Heq2' := Heq2).
+    apply (appears_false_remove _ _ (p⊗q)) in Heq2.
+    apply in_not_exists_in_env.
+    intros φ H3.
+    assert (appears true n (p⊗q) = false) by
+      (apply not_exists_in_env_in with (Γ:=Γ);assumption).
+    simpl in H0.
+    rewrite Bool.orb_false_iff in H0;intuition.
+    destruct (mem_destruct _ _ _ H3) as [H5|H5].
+    apply eq_is_eq in H5;subst;assumption.
+    destruct (mem_destruct _ _ _ H5) as [H6|H6].
+    apply eq_is_eq in H6;subst;assumption.
+    apply not_exists_in_env_in with (Γ:=Γ\p⊗q); assumption.
+
+    Focus.
+    apply IHILL_proof.
+    assumption.
+    assert (Heq2' := Heq2).
+    apply (appears_false_remove _ _ 1) in Heq2.
+    assumption.
+
+    Focus.
+    rewrite Bool.orb_true_iff in Heq1;destruct Heq1; eauto.
+
+    Focus.
+    apply IHILL_proof.
+    assumption.
+    assert (Heq2' := Heq2).
+    apply (appears_false_remove _ _ (p&q)) in Heq2.
+    apply in_not_exists_in_env.
+    intros φ H3.
+    assert (appears true n (p&q) = false) by
+      (apply not_exists_in_env_in with (Γ:=Γ);assumption).
+    simpl in H0.
+    rewrite Bool.orb_false_iff in H0;intuition.
+    destruct (mem_destruct _ _ _ H3) as [H5|H5].
+    apply eq_is_eq in H5;subst;assumption.
+    apply not_exists_in_env_in with (Γ:=Γ\p&q); assumption.
+
+    Focus.
+    apply IHILL_proof.
+    assumption.
+    assert (Heq2' := Heq2).
+    apply (appears_false_remove _ _ (p&q)) in Heq2.
+    apply in_not_exists_in_env.
+    intros φ H3.
+    assert (appears true n (p&q) = false) by
+      (apply not_exists_in_env_in with (Γ:=Γ);assumption).
+    simpl in H0.
+    rewrite Bool.orb_false_iff in H0;intuition.
+    destruct (mem_destruct _ _ _ H3) as [H5|H5].
+    apply eq_is_eq in H5;subst;assumption.
+    apply not_exists_in_env_in with (Γ:=Γ\p&q); assumption.
+
+    Focus.
+    apply IHILL_proof1.
+    assumption.
+    assert (Heq2' := Heq2).
+    apply (appears_false_remove _ _ (p⊕q)) in Heq2.
+    apply in_not_exists_in_env.
+    intros φ H3.
+    assert (appears true n (p⊕q) = false) by
+      (apply not_exists_in_env_in with (Γ:=Γ);assumption).
+    simpl in H0.
+    rewrite Bool.orb_false_iff in H0;intuition.
+    destruct (mem_destruct _ _ _ H3) as [H5|H5].
+    apply eq_is_eq in H5;subst;assumption.
+    apply not_exists_in_env_in with (Γ:=Γ\p⊕q); assumption.
+
+    Focus.
+    assert (H':=  not_exists_in_env_in _ _ Heq2).
+    generalize (H' _ H).
+    simpl;discriminate.
+
+    Focus.
+    apply IHILL_proof.
+    assumption.
+    assert (Heq2' := Heq2).
+    apply (appears_false_remove _ _ (!p)) in Heq2.
+    apply in_not_exists_in_env.
+    intros φ H3.
+    assert (appears true n (!p) = false) by
+      (apply not_exists_in_env_in with (Γ:=Γ);assumption).
+    simpl in H0.
+    destruct (mem_destruct _ _ _ H3) as [H5|H5].
+    apply eq_is_eq in H5;subst;assumption.
+    apply not_exists_in_env_in with (Γ:=Γ\!p); assumption.
+
+    Focus.
+    apply IHILL_proof.
+    assumption.
+    assert (Heq2' := Heq2).
+    apply (appears_false_remove _ _ (!p)) in Heq2.
+    apply in_not_exists_in_env.
+    intros φ H3.
+    assert (appears true n (!p) = false) by
+      (apply not_exists_in_env_in with (Γ:=Γ);assumption).
+    simpl in H0.
+    destruct (mem_destruct _ _ _ H3) as [H5|H5].
+    apply eq_is_eq in H5;subst;assumption.
+    apply not_exists_in_env_in with (Γ:=Γ); assumption.
+
+    Focus.
+    apply IHILL_proof.
+    assumption.
+    assert (Heq2' := Heq2).
+    apply (appears_false_remove _ _ (!p)) in Heq2.
+    apply in_not_exists_in_env.
+    intros φ H3.
+    assert (appears true n (!p) = false) by
+      (apply not_exists_in_env_in with (Γ:=Γ);assumption).
+    simpl in H0.
+    apply not_exists_in_env_in with (Γ:=Γ\!p); assumption.
+  Qed.  
+
+  Function sub_formula (n : nat) (ψ:formula) {struct ψ} : bool :=
+    match ψ with 
+      | Proposition m => EqNat.beq_nat n m
+      | f1 ⊸ f2 | f1 ⊕ f2 | f1 ⊗ f2 | f1 & f2 => orb (sub_formula n f1) (sub_formula n f2)
+      | !f => sub_formula n f
+      | Top => true
+      | Zero => true
+      | _ => false
+    end.
+
+  Function in_lhs_arrow (p: formula -> bool) (φ:formula) {struct φ} : bool :=
+    match φ with 
+      | f1 ⊕ f2 | f1 ⊗ f2 | f1 & f2 => orb (in_lhs_arrow p f1) (in_lhs_arrow p f2)
+      | !f => in_lhs_arrow p f
+      | (f1 ⊸ f2) => orb (p f1) (in_lhs_arrow p f2)
+      | Zero => true
+      | _ => false
+    end.
+
+
+  Lemma not_sub_not_in_lhs_arrow : forall n φ, sub_formula n φ = false -> in_lhs_arrow (sub_formula n) φ = false.
+  Proof.
+    intros n φ.
+    functional induction (sub_formula n φ);simpl;try reflexivity.
+
+    Focus.
+    intros Hsub;  rewrite Bool.orb_false_iff in Hsub;destruct Hsub.
+    rewrite H.
+    rewrite IHb0 by assumption.
+    reflexivity.
+
+    Focus.
+    intros Hsub;  rewrite Bool.orb_false_iff in Hsub;destruct Hsub.
+    rewrite IHb by assumption.
+    rewrite IHb0 by assumption.
+    reflexivity.
+
+    Focus.
+    intros Hsub;  rewrite Bool.orb_false_iff in Hsub;destruct Hsub.
+    rewrite IHb by assumption.
+    rewrite IHb0 by assumption.
+    reflexivity.
+
+    Focus.
+    intros Hsub;  rewrite Bool.orb_false_iff in Hsub;destruct Hsub.
+    rewrite IHb by assumption.
+    rewrite IHb0 by assumption.
+    reflexivity.
+
+    Focus.
+    assumption.
+
+    Focus. discriminate.
+
+    Focus.
+    destruct ψ;  try reflexivity;try tauto.
+  Qed.
+
+  Lemma var_not_in_env:  ∀ Γ φ n,  (Proposition n)∈Γ -> (sub_formula n φ) = false ->  ~FormulaOrdered.eq φ (⊤) ->
+    (forall ψ, ψ∈Γ -> (in_lhs_arrow (sub_formula n) ψ) = false) ->  Γ⊢φ -> False.
+  Proof.  
+    intros Γ φ n H H0 H1 H2 H3.
+    revert H H0 H1 H2.
+
+    induction H3;intros  Hin Hsub Hnottop Hall ;simpl in *;try discriminate.
+
+    Focus.
+    rewrite H in  Hin.
+    destruct (mem_destruct _ _ _ Hin) as [H1|H1].
+    apply eq_is_eq in H1;subst p;simpl in Hsub.
+    rewrite <- EqNat.beq_nat_refl in Hsub;discriminate.
+    unfold mem in H1.
+    rewrite MapsPtes.F.empty_a in H1;discriminate.
+
+    Focus.
+    rewrite Bool.orb_false_iff in Hsub;destruct Hsub.
+    clear Hnottop.
+    apply IHILL_proof.
+    apply mem_add_comm;assumption.
+    assumption.
+    destruct q;simpl;intros;try tauto.
+    simpl in H0;discriminate.
+    intros ψ H1.
+    destruct (mem_destruct _ _ _ H1) as [H4|H4];clear H1.
+    apply eq_is_eq in H4;subst p.
+    apply not_sub_not_in_lhs_arrow;assumption.
+    auto.
+
+    Focus.
+    rewrite mem_remove_1 with (b:=p ⊸ q) in Hin by (intros abs; apply eq_is_eq in abs;discriminate).
+    rewrite H0 in Hin.
+    assert (sub_formula n p =false /\ in_lhs_arrow (sub_formula n) q = false ). 
+    generalize (Hall _ H);  simpl. 
+    intro H3; rewrite Bool.orb_false_iff in H3;assumption.
+    destruct H1.
+    destruct (mem_union_destruct _ _ _ Hin) as [H3|H3].
+    apply IHILL_proof1;try assumption.
+    destruct p;simpl;try tauto.
+    simpl in H1;discriminate.
+    intros ψ H4.
+    apply Hall.
+    apply mem_remove_2 with (p⊸q).
+    rewrite H0.
+    auto using mem_union_l.
+    apply IHILL_proof2;try assumption.
+    apply mem_add_comm;assumption.  
+    intros ψ H4.
+    destruct (mem_destruct _ _ _ H4) as [H5|H5].
+    apply eq_is_eq in H5;subst;assumption.
+    apply Hall.
+    apply mem_remove_2 with (p⊸q).
+    rewrite H0.
+    auto using mem_union_r.
+
+    Focus.
+    assert (Hin' := Hin).
+    rewrite H in Hin.
+    rewrite Bool.orb_false_iff in Hsub;destruct Hsub.
+    destruct (mem_union_destruct _ _ _ Hin) as [H3|H3].
+    apply IHILL_proof1;try assumption.
+    destruct p;simpl;try tauto.
+    simpl in H1;discriminate.
+    intros ψ H4.
+    apply Hall.
+    rewrite H.
+    auto using mem_union_l.
+    apply IHILL_proof2;try assumption.
+    destruct q;simpl;try tauto.
+    simpl in H1;discriminate.
+    intros ψ H4.
+    apply Hall.
+    rewrite H.
+    auto using mem_union_r.
+
+    Focus.
+    assert (Hin' := Hin).
+    apply IHILL_proof;try assumption.
+    do 2 (apply mem_add_comm).
+    rewrite mem_remove_1  with (b:=p ⊗ q) in Hin by (intros abs; apply eq_is_eq in abs;discriminate).
+    assumption.
+    assert (in_lhs_arrow (sub_formula n) p =false /\ in_lhs_arrow (sub_formula n) q = false ). 
+    generalize (Hall _ H);  simpl. 
+    intro H4; rewrite Bool.orb_false_iff in H4;assumption.
+    destruct H0.
+    intros ψ H4.
+    destruct (mem_destruct _ _ _ H4) as [H5|H5].
+    apply eq_is_eq in H5;subst;assumption.
+    destruct (mem_destruct _ _ _ H5) as [H6|H6].
+    apply eq_is_eq in H6;subst;assumption.
+    apply Hall.
+    eapply mem_remove_2;eassumption.
+
+    Focus.
+    rewrite H in Hin.
+    unfold mem in Hin.
+    rewrite MapsPtes.F.empty_a in Hin;discriminate.
+
+    Focus.
+    assert (Hin' := Hin).
+    apply IHILL_proof;try assumption.
+    rewrite mem_remove_1  with (b:=1) in Hin by (intros abs; apply eq_is_eq in abs;discriminate).
+    assumption.
+    intros ψ H0.
+    apply Hall.
+    eapply mem_remove_2;eassumption.
+
+
+    Focus.
+    assert (Hin' := Hin).
+    rewrite Bool.orb_false_iff in Hsub;destruct Hsub.
+    apply IHILL_proof1;try assumption.
+    destruct q;simpl;try tauto.
+    simpl in H;discriminate.
+
+    Focus.
+    assert (Hin' := Hin).
+    apply IHILL_proof;try assumption.
+    do 1 (apply mem_add_comm).
+    rewrite mem_remove_1  with (b:=p & q) in Hin by (intros abs; apply eq_is_eq in abs;discriminate).
+    assumption.
+    assert (in_lhs_arrow (sub_formula n) p =false /\ in_lhs_arrow (sub_formula n) q = false ). 
+    generalize (Hall _ H);  simpl. 
+    intro H4; rewrite Bool.orb_false_iff in H4;assumption.
+    destruct H0.
+    intros ψ H4.
+    destruct (mem_destruct _ _ _ H4) as [H5|H5].
+    apply eq_is_eq in H5;subst;assumption.
+    apply Hall.
+    eapply mem_remove_2;eassumption.
+
+    Focus.
+    assert (Hin' := Hin).
+    apply IHILL_proof;try assumption.
+    do 1 (apply mem_add_comm).
+    rewrite mem_remove_1  with (b:=p & q) in Hin by (intros abs; apply eq_is_eq in abs;discriminate).
+    assumption.
+    assert (in_lhs_arrow (sub_formula n) p =false /\ in_lhs_arrow (sub_formula n) q = false ). 
+    generalize (Hall _ H);  simpl. 
+    intro H4; rewrite Bool.orb_false_iff in H4;assumption.
+    destruct H0.
+    intros ψ H4.
+    destruct (mem_destruct _ _ _ H4) as [H5|H5].
+    apply eq_is_eq in H5;subst;assumption.
+    apply Hall.
+    eapply mem_remove_2;eassumption.
+
+
+    Focus.
+    assert (Hin' := Hin).
+    apply IHILL_proof1;try assumption.
+    do 1 (apply mem_add_comm).
+    rewrite mem_remove_1  with (b:=p ⊕ q) in Hin by (intros abs; apply eq_is_eq in abs;discriminate).
+    assumption.
+    assert (in_lhs_arrow (sub_formula n) p =false /\ in_lhs_arrow (sub_formula n) q = false ). 
+    generalize (Hall _ H);  simpl. 
+    intro H3; rewrite Bool.orb_false_iff in H3;assumption.
+    destruct H0.
+    intros ψ H3.
+    destruct (mem_destruct _ _ _ H3) as [H4|H4].
+    apply eq_is_eq in H4;subst;assumption.
+    apply Hall.
+    eapply mem_remove_2;eassumption.
+
+    Focus.
+    assert (Hin' := Hin).
+    rewrite Bool.orb_false_iff in Hsub;destruct Hsub.
+    apply IHILL_proof;try assumption.
+    destruct p;simpl;try tauto.
+    simpl in H;discriminate.
+
+    Focus.
+    assert (Hin' := Hin).
+    rewrite Bool.orb_false_iff in Hsub;destruct Hsub.
+    apply IHILL_proof;try assumption.
+    destruct q;simpl;try tauto.
+    simpl in H;discriminate.
+
+
+    Focus.
+    generalize (Hall _ H); simpl;discriminate.
+
+    Focus.
+    apply IHILL_proof;try assumption.
+    apply mem_add_comm.
+    rewrite <- mem_remove_1 with (b:=!p) by (intros abs; apply eq_is_eq in abs;discriminate).
+    assumption.
+    intros ψ H0.
+    destruct (mem_destruct _ _ _ H0) as [H2|H2];clear H0.
+    apply eq_is_eq in H2;subst. 
+    generalize (Hall _ H);simpl;tauto.
+    apply Hall.
+    eapply mem_remove_2;eassumption. 
+
+    Focus.
+    apply IHILL_proof;try assumption.
+    apply mem_add_comm;assumption.
+    intros ψ H0.
+    destruct (mem_destruct _ _ _ H0) as [H2|H2];clear H0.
+    apply eq_is_eq in H2;subst. 
+    generalize (Hall _ H);simpl;tauto.
+    apply Hall;assumption.
+
+    Focus.
+    apply IHILL_proof;try assumption.
+    rewrite <- mem_remove_1 by (intros abs; apply eq_is_eq in abs;discriminate).
+    assumption.
+    intros ψ H0.
+    apply Hall.
+    eapply mem_remove_2;eassumption. 
+  Qed.  
+
+  Lemma ILL_proof_pre_morph' : 
+    ∀ (φ : formula) (Γ Γ' : t), Γ ⊢ φ → eq_bool Γ  Γ' = true → Γ' ⊢ φ.
+  Proof.
+    intros φ Γ Γ' H H0.
+    eapply ILL_proof_pre_morph;try eassumption.
+    apply eq_bool_correct;assumption.
+  Qed.
+  Hint Resolve ILL_proof_pre_morph' : proof.
 
 
 End M.
